progs/message.v
@@ -88,10 +88,12 @@ Definition f_intpair_deserialize := {|
         (Efield
           (Ederef (Etempvar _p (tptr t_struct_intpair)) t_struct_intpair) _x
           tint) (Etempvar _x tint))
-      (Sassign
-        (Efield
-          (Ederef (Etempvar _p (tptr t_struct_intpair)) t_struct_intpair) _y
-          tint) (Etempvar _y tint)))))
+      (Ssequence
+        (Sassign
+          (Efield
+            (Ederef (Etempvar _p (tptr t_struct_intpair)) t_struct_intpair)
+            _y tint) (Etempvar _y tint))
+        (Sreturn None)))))
 |}.
 
 Definition v_intpair_message := {|
