progs/verif_message.v
@@ -36,15 +36,16 @@ Definition serialize_spec {t: type} (format: message_format t) :=
            * `(format sh' buf) (`Int.unsigned (`force_int retval)) `data.
 
 Definition deserialize_spec {t: type} (format: message_format t) :=
-  WITH data: reptype t, p: val, buf: val, sh: share, sh': share
+  WITH data: reptype t, p: val, buf: val, shs: share*share, len: Z
   PRE [ _p OF (tptr t), _buf OF (tptr tuchar), _length OF tint ] 
-          PROP (writable_share sh)
-          LOCAL (`(eq p) (eval_id _p); `(eq buf) (eval_id _buf))
-          SEP (`(format sh' buf) (`Int.unsigned (`force_int (eval_id _length))) `data;
-                 `(memory_block sh' (Int.repr (sizeof t)) p))
+          PROP (writable_share (fst shs))
+          LOCAL (`(eq p) (eval_id _p); `(eq buf) (eval_id _buf);
+                        `(eq (Vint (Int.repr len))) (eval_id _length))
+          SEP (`(format (snd shs) buf len) `data;
+                 `(memory_block (fst shs) (Int.repr (sizeof t)) p))
   POST [ tint ]
-            `(format sh' buf) (`Int.unsigned (`force_int (eval_id _length))) `data *
-            `(typed_mapsto t sh p data).
+            `(format (snd shs) buf len data) *
+            `(typed_mapsto t (fst shs) p data).
 
 Definition intpair_serialize_spec :=
  DECLARE _intpair_serialize (serialize_spec intpair_message).
@@ -121,7 +122,131 @@ apply sepcon_derives; apply derives_refl';
 destruct buf0; inv H0; reflexivity.
 Qed.
 
+Lemma body_intpair_deserialize: semax_body Vprog Gtot f_intpair_deserialize intpair_deserialize_spec.
+Proof.
+unfold intpair_deserialize_spec, deserialize_spec.
+start_function. destruct shs as (sh,sh'). simpl @fst; simpl @snd.
+name p0 _p.
+name buf0 _buf.
+name x _x.
+name y _y.
+name len0 _length.
+rewrite memory_block_typed.
+do 2 simpl_typed_mapsto.
+destruct data as (x1,y1); simpl in *.
+apply semax_pre_PQR with
+ (PROP  (isptr buf; len=8)
+   LOCAL  (`(eq p) (eval_id _p); `(eq buf) (eval_id _buf); `(eq (Vint (Int.repr len))) (eval_id _length))
+   SEP 
+   (`(field_mapsto_ sh t_struct_intpair _x) (eval_id _p);
+    `(field_mapsto_ sh t_struct_intpair _y) (eval_id _p);
+   `(mapsto sh' tint)
+        (`(add_ptr_int tint) (`(eval_cast (tptr tuchar) (tptr tint)) (eval_id _buf)) `0)
+      `(Vint x1);
+   `(mapsto sh' tint)
+        (`(add_ptr_int tint) (`(eval_cast (tptr tuchar) (tptr tint)) (eval_id _buf)) `1)
+        `(Vint y1))).
+go_lower; subst. unfold intpair_message.
+ simpl_typed_mapsto.  rewrite (field_mapsto_isptr). normalize. 
+ cancel.
+apply sepcon_derives; apply derives_refl'';
+ eapply mapsto_field_mapsto; unfold field_offset; try (simpl; reflexivity);
+ apply add_ptr_int_offset;
+ simpl; compute; intuition congruence.
+normalizex.
+forward. (* x = ((int * )buf)[0]; *)
+go_lower. subst buf0 p0. apply prop_right; auto. 
+forward. (* y = ((int * )buf)[1]; *)
+go_lower. subst buf0 p0. apply prop_right; auto. 
+forward. (* p->x = x; *)
+forward. (*  p->y = y; *)
+forward.  (* return; *)
+go_lower. subst. unfold intpair_message. normalize.
+simpl_typed_mapsto.
+cancel.
+simpl. rewrite sepcon_comm.
+apply sepcon_derives;
+apply derives_refl'; eapply mapsto_field_mapsto;  unfold field_offset; try (simpl; reflexivity);
+ destruct buf0; inv H0; reflexivity.
+Qed.
 
+
+Ltac start_function := 
+ match goal with |- semax_body _ _ _ ?spec => try unfold spec end;
+ match goal with |- semax_body _ _ _ (pair _ (mk_funspec _ _ ?Pre _)) =>
+   match Pre with 
+   | (fun x => match x with (a,b) => _ end) => intros [a b] 
+   | (fun i => _) => intro i
+   end;
+   simpl fn_body; simpl fn_params; simpl fn_return
+ end;
+ repeat match goal with |- semax _ (match ?p with (a,b) => _ end * _) _ _ =>
+             destruct p as [a b]
+           end;
+ match goal with |- semax (func_tycontext ?F ?V ?G) _ _ _ => 
+   set (Delta := func_tycontext F V G)
+ end;
+  match goal with
+  | |- semax _ (?P * stackframe_of ?F) _ _ =>
+            change (stackframe_of F) with (@emp assert _ _);
+            rewrite sepcon_emp;
+            rewrite frame_ret_assert_emp
+  | |- semax _ ((PROPx ?P (LOCALx ?Q (SEPx ?R))) * stackframe_of ?F) _ _ =>
+        change (@LiftNatDed environ mpred Nveric) with Nassert;
+        change (@LiftSepLog environ mpred Nveric Sveric) with Sassert;
+        rewrite (start_function_aux1 (stackframe_of F) P Q R)
+ | |- _ => idtac
+  end;
+ match goal with
+  | |- semax _ (PROPx _ _) _ _ => idtac 
+  | _ => canonicalize_pre 
+ end;
+ repeat (apply semax_extract_PROP; intro).
+
+
+Lemma memory_block_isptr: forall sh i v, 
+  i > 0 -> 
+  memory_block sh (Int.repr i) v = !!(isptr v) && memory_block sh (Int.repr i) v.
+Proof.
+Admitted.  (* not difficult *)
+
+Lemma typed_mapsto__isptr:
+  forall sh t v, typed_mapsto_ sh t v = !!(isptr v) && typed_mapsto_ sh t v.
+Proof.
+intros.
+rewrite <- memory_block_typed.
+apply memory_block_isptr.
+apply sizeof_pos.
+Qed.
+
+Lemma var_block_typed_mapsto_:
+  forall  sh id t, 
+ var_block sh (id, t) = `(typed_mapsto_ (Share.splice sh Share.top) t) (eval_var id t).
+Proof.
+intros; extensionality rho.
+unfold_coerce.
+rewrite <- memory_block_typed.
+unfold var_block, lvalue_block.
+rewrite memory_block_isptr by apply sizeof_pos.
+simpl.
+destruct (eval_var id t rho); simpl; normalize.
+Admitted.
+
+
+Lemma var_block_typed_mapsto__top:
+  forall id t, 
+ var_block Share.top (id, t) = `(typed_mapsto_ Share.top t) (eval_var id t).
+Proof.
+intros.
+rewrite var_block_typed_mapsto_.
+rewrite splice_top_top; auto.
+Qed.
+
+Lemma body_main:  semax_body Vprog Gtot f_main main_spec.
+Proof.
+start_function.
+unfold stackframe_of, fn_vars. simpl map. unfold fold_right.
+repeat rewrite var_block_typed_mapsto__top.
 
 
 
